examples/cnf/dist/array/distrup_listScript.sml
@@ -7,92 +7,110 @@ Ancestors
 Libs
   preamble
 
-Definition resize_dm_def:
-  resize_dm dml b v =
-  let lv = length v in
-  let sz = sz_lit_map lv v 0 in
-  reset_dm_list dml b sz
+(* TODO: move to ccnf_list and
+  rename everything consistently *)
+Definition unit_prop_one_def:
+  unit_prop_one fml dml b i =
+  case FLOOKUP fml i of
+    NONE => NONE
+  | SOME c =>
+    delete_literals_sing_list dml b c (length c)
 End
 
-Theorem bnd_clause_resize_dm:
-  resize_dm dml b v = (dml',b') ⇒
-  bnd_clause v (LENGTH dml')
+Definition unit_prop_list_def:
+  (unit_prop_list fml dml b [] = SOME (F,dml)) ∧
+  (unit_prop_list fml dml b (i::is) =
+  case unit_prop_one fml dml b i of
+    NONE => NONE
+  | SOME (T,dml') => SOME (T,dml')
+  | SOME (F,dml') => unit_prop_list fml dml' b is)
+End
+
+Definition is_rup_list_def:
+  is_rup_list fml dml b v is =
+  let (dml',b') = prepare_rup dml b v in
+  case unit_prop_list fml dml' b' is of
+    SOME (T,dml'') => (T,dml'',b')
+  | _ => (F, (dml',b'))
+End
+
+Theorem is_rup_list:
+  dm_rel dm dml b ∧
+  is_rup_list fml dml b v is = (T, (dml',b')) ⇒
+  is_rup fml v is ∧
+  ∃dm'. dm_rel dm' dml' b'
 Proof
-  rw[resize_dm_def]>>
-  irule bnd_clause_le >>
-  gvs[reset_dm_list_def,AllCaseEqs(),NOT_LESS] >>
-  irule_at (Pos last) sz_lit_map_bnd_clause >>
-  Q.EXISTS_TAC `0` >> fs[]
+  cheat
 QED
 
-Theorem resize_dm_LENGTH:
-  resize_dm dml b v = (dml',b') ⇒
-  LENGTH dml ≤ LENGTH dml'
-Proof
-  rw[resize_dm_def]>>
-  drule_then strip_assume_tac reset_dm_list_LENGTH
-QED
+Definition bnd_fml_def:
+  bnd_fml fml sz ⇔
+  ∀v.
+    v ∈ FRANGE fml ⇒
+    bnd_clause v sz
+End
+
+(* END MOVE *)
 
 (* Refinement to make use of array representations *)
 Definition check_distrup_list_def:
   check_distrup_list distrup fml dml b =
   case distrup of
   | Del ls =>
-    SOME (delete_ids_list fml ls, (dml, b))
+    SOME (delete_ids fml ls, (dml, b))
   | Lrup n vc hints =>
     (case is_rup_list fml dml b vc hints of
       (T, dmlb) =>
-      SOME (update_resize fml NONE (SOME vc) n, dmlb)
+      SOME (fml |+ (n, vc) , dmlb)
     | _ => NONE)
   | Import n vc =>
-      SOME (update_resize fml NONE (SOME vc) n, resize_dm dml b vc)
+      SOME (fml |+ (n, vc) , resize_dm dml b vc)
   | ValidateUnsat =>
-    if contains_emp_list fml then
+    if contains_emp fml then
       SOME (fml, (dml,b))
     else NONE
 End
 
 Theorem check_distrup_list:
-  fml_rel fml fmlls ∧
   dm_rel dm dml b ∧
-  check_distrup_list distrup fmlls dml b = SOME (fmlls',(dml',b')) ⇒
-  ∃fml' dm'.
+  check_distrup_list distrup fml dml b =
+    SOME (fml',(dml',b')) ⇒
+  ∃dm'.
     check_distrup distrup fml = SOME fml' ∧
-    fml_rel fml' fmlls' ∧
     dm_rel dm' dml' b'
 Proof
   simp[check_distrup_list_def]>>strip_tac>>
   gvs[AllCaseEqs(),check_distrup_def]
-  >- (simp[fml_rel_delete_ids_list]>>metis_tac[])
+  >- metis_tac[]
   >- (
-    drule_all is_rup_list>>rw[]>>
-    simp[fml_rel_update_resize]>>
-    metis_tac[])
+    drule_all is_rup_list>>rw[])
   >- (
-    simp[fml_rel_update_resize]>>
     gvs[resize_dm_def]>>
     drule_all dm_rel_reset_dm_list>>
     metis_tac[])
   >-
-    metis_tac[fml_rel_contains_emp_list]
+    metis_tac[]
 QED
 
 Theorem check_distrup_list_bnd_fml:
-  bnd_fml fmlls (LENGTH dml) ∧
-  check_distrup_list distrup fmlls dml b = SOME (fmlls',(dml',b')) ⇒
-  bnd_fml fmlls' (LENGTH dml')
+  bnd_fml fml (LENGTH dml) ∧
+  check_distrup_list distrup fml dml b = SOME (fml',(dml',b')) ⇒
+  bnd_fml fml' (LENGTH dml')
 Proof
   simp[check_distrup_list_def]>>strip_tac>>
   gvs[AllCaseEqs(),check_distrup_def]
-  >- metis_tac[bnd_fml_delete_ids_list]
+  >- cheat (* metis_tac[bnd_fml_delete_ids_list] *)
   >- (
-    drule_all bnd_fml_is_rup_list>>
-    metis_tac[bnd_fml_update_resize])
+    cheat
+    (* drule_all bnd_fml_is_rup_list>>
+    metis_tac[bnd_fml_update_resize]*))
   >- (
+    cheat
+    (*
     irule bnd_fml_update_resize>>
     drule bnd_clause_resize_dm>>
     simp[]>>
     rw[]>>irule bnd_fml_le>>
-    metis_tac[resize_dm_LENGTH])
+    metis_tac[resize_dm_LENGTH]*))
 QED
 
